src/program_proof/pav/phys_hist.v
@@ -1,0 +1,99 @@
+From Perennial.program_proof.pav Require Import prelude.
+From Goose.github_com.mit_pdos.pav Require Import kt.
+
+From Perennial.program_proof.pav Require Import core serde.
+
+Section wps.
+Context `{!heapGS Σ, !pavG Σ}.
+
+Definition is_HistEntry (ptr : loc) (obj : map_val_ty) : iProp Σ :=
+  ∃ sl_HistVal,
+  "#Hptr_Epoch" ∷ ptr ↦[HistEntry :: "Epoch"]□ #obj.1 ∗
+  "#Hptr_HistVal" ∷ ptr ↦[HistEntry :: "HistVal"]□ (slice_val sl_HistVal) ∗
+  "#Hsl_HistVal" ∷ own_slice_small sl_HistVal byteT DfracDiscarded obj.2.
+
+Definition own_hist sl_hist hist : iProp Σ :=
+  ∃ dim0_hist,
+  "Hsl_hist" ∷ own_slice sl_hist ptrT (DfracOwn 1) dim0_hist ∗
+  "#Hdim0_hist" ∷ ([∗ list] p;o ∈ dim0_hist;hist, is_HistEntry p o).
+
+Lemma wp_put_hist sl_hist hist ptr_e ep pk  :
+  {{{
+    "Hown_hist" ∷ own_hist sl_hist hist ∗
+    "#His_entry" ∷ is_HistEntry ptr_e (ep, pk)
+  }}}
+  SliceAppend ptrT (slice_val sl_hist) #ptr_e
+  {{{
+    sl_hist', RET (slice_val sl_hist');
+    "Hown_hist" ∷ own_hist sl_hist' (hist ++ [(ep, pk)])
+  }}}.
+Proof.
+  iIntros (Φ) "H HΦ". iNamed "H". iNamed "Hown_hist".
+  wp_apply (wp_SliceAppend with "Hsl_hist"). iIntros (?) "Hsl_hist".
+  iDestruct (big_sepL2_snoc with "[$Hdim0_hist $His_entry]") as "Hnew_dim0_hist".
+  iApply "HΦ". iFrame "∗#".
+Qed.
+
+Lemma wp_GetHist sl_hist hist (ep : w64) :
+  {{{
+    "Hown_hist" ∷ own_hist sl_hist hist
+  }}}
+  GetHist (slice_val sl_hist) #ep
+  {{{
+    (is_reg : bool) sl_pk pk, RET (#is_reg, slice_val sl_pk);
+    "Hown_hist" ∷ own_hist sl_hist hist ∗
+    "#Hsl_pk" ∷ own_slice_small sl_pk byteT DfracDiscarded pk ∗
+    "%Heq_lat" ∷
+      ⌜ match get_lat hist ep with
+        | None => is_reg = false
+        | Some lat => is_reg = true ∧ pk = lat.2
+        end ⌝
+  }}}.
+Proof.
+  iIntros (Φ) "H HΦ". iNamed "H". rewrite /GetHist. iNamed "Hown_hist".
+  wp_apply wp_ref_of_zero; [done|]. iIntros (ptr_isReg) "Hptr_isReg".
+  wp_apply wp_ref_of_zero; [done|]. iIntros (ptr_val) "Hptr_val".
+  iDestruct (own_slice_small_read with "Hsl_hist") as "[Hsl_hist Hsl_restore]".
+  wp_apply (wp_forSlicePrefix
+    (λ donel _,
+    ∃ (is_reg : bool) sl_pk pk,
+    "Hptr_isReg" ∷ ptr_isReg ↦[boolT] #is_reg ∗
+    "Hptr_val" ∷ ptr_val ↦[slice.T byteT] (slice_val sl_pk) ∗
+    "Hsl_pk" ∷ own_slice_small sl_pk byteT DfracDiscarded pk ∗
+    "%Heq_lat" ∷
+      ⌜ match get_lat (take (length donel) hist) ep with
+        | None => is_reg = false
+        | Some lat => is_reg = true ∧ pk = lat.2
+        end ⌝)%I with "[] [$Hsl_hist Hptr_isReg Hptr_val]").
+  2: { iExists _, Slice.nil, []. iFrame. iSplit; [|done].
+    iDestruct (own_slice_zero byteT) as "H".
+    by iDestruct (own_slice_to_small with "H") as "?". }
+  { clear. iIntros "* %". iIntros (Φ) "!> H HΦ". iNamed "H".
+    opose proof (list_lookup_middle done todo x _ _) as Hlook_x; [done|].
+    subst dim0_hist.
+    iDestruct (big_sepL2_lookup_1_some with "Hdim0_hist")
+      as %[[new_ep new_pk] Hlook_hist]; [exact Hlook_x|].
+    iDestruct (big_sepL2_lookup with "Hdim0_hist")
+      as "His_entry"; [exact Hlook_x|exact Hlook_hist|].
+    iNamed "His_entry". wp_loadField. wp_if_destruct.
+    - wp_store. wp_loadField. wp_store. iApply "HΦ".
+      iFrame "Hsl_HistVal". iFrame "∗#". rewrite app_length. simpl.
+      replace (length done + 1)%nat with (S $ length done)%nat; [|lia].
+      rewrite (take_S_r _ _ _ Hlook_hist). rewrite /get_lat filter_app.
+      opose proof (list_filter_singleton (λ x, uint.Z x.1 ≤ uint.Z ep)
+        (new_ep, new_pk)) as [[_?]|[Htmp _]]. { exfalso. simpl in *. word. }
+      rewrite Htmp. clear Htmp. rewrite last_snoc. naive_solver.
+    - iApply "HΦ". iFrame "Hsl_pk". iFrame "∗#". rewrite app_length. simpl.
+      replace (length done + 1)%nat with (S $ length done)%nat; [|lia].
+      rewrite (take_S_r _ _ _ Hlook_hist). rewrite /get_lat filter_app.
+      opose proof (list_filter_singleton (λ x, uint.Z x.1 ≤ uint.Z ep)
+        (new_ep, new_pk)) as [[Htmp _]|[_?]]. 2: { exfalso. simpl in *. word. }
+      rewrite Htmp. clear Htmp. list_simplifier. by iFrame "%". }
+  iIntros "[H0 H1]". iNamed "H1". iDestruct ("Hsl_restore" with "H0") as "Hsl_hist".
+  do 2 wp_load. wp_pures. iApply "HΦ". iFrame "∗#".
+  iDestruct (big_sepL2_length with "Hdim0_hist") as %Htmp.
+  rewrite Htmp in Heq_lat. clear Htmp.
+  rewrite firstn_all in Heq_lat. naive_solver.
+Qed.
+
+End wps.
